Changed abstraction of CC, added input to the data structure, added invariants

Congruence_Closure_Explain/CC_Abstraction.thy
@@ -4,30 +4,60 @@ begin
 
 section \<open>Abstract formalisation of congruence closure\<close>
 
-datatype equation_term = Apply equation_term equation_term | Symb nat
-
 
 text \<open>S is the set of input equations.
 The Congruence Closure is the smallest relation that includes S and is closed under reflexivity,
 symmetry, transitivity, and under function application.
 Source: \<open>https://drops.dagstuhl.de/opus/volltexte/2021/14253/pdf/LIPIcs-FSCD-2021-15.pdf\<close>\<close>
 
-inductive Congruence_Closure :: "(equation_term * equation_term) set \<Rightarrow> (equation_term * equation_term) \<Rightarrow> bool"
+inductive Congruence_Closure :: "equation set \<Rightarrow> equation \<Rightarrow> bool"
   where
 base: "eqt \<in> S \<Longrightarrow> Congruence_Closure S eqt"
-| reflexive: "Congruence_Closure S (a, a)"
-| symmetric: "Congruence_Closure S (a, b) \<Longrightarrow> Congruence_Closure S (b, a)"
-| transitive: "Congruence_Closure S (a, b) \<Longrightarrow> Congruence_Closure S (b, c) \<Longrightarrow> Congruence_Closure S (a, c)"
-| monotonic: "Congruence_Closure S (a\<^sub>1, b\<^sub>1) \<Longrightarrow> Congruence_Closure S (a\<^sub>2, b\<^sub>2) \<Longrightarrow> Congruence_Closure S ((Apply a\<^sub>1 a\<^sub>2), (Apply b\<^sub>1 b\<^sub>2))"
+| reflexive: "Congruence_Closure S (a \<approx> a)"
+| symmetric: "Congruence_Closure S (a \<approx> b) \<Longrightarrow> Congruence_Closure S (b \<approx> a)"
+| transitive: "Congruence_Closure S (a \<approx> b) \<Longrightarrow> Congruence_Closure S (b \<approx> c) \<Longrightarrow> Congruence_Closure S (a \<approx> c)"
+| monotonic: "Congruence_Closure S (F a\<^sub>1 a\<^sub>2 \<approx> a) \<Longrightarrow> Congruence_Closure S (F b\<^sub>1 b\<^sub>2 \<approx> b) 
+\<Longrightarrow> Congruence_Closure S (a\<^sub>1 \<approx> b\<^sub>1) \<Longrightarrow> Congruence_Closure S (a\<^sub>2 \<approx> b\<^sub>2)
+\<Longrightarrow> Congruence_Closure S (a \<approx> b)"
 
-fun equation_\<alpha> :: "equation \<Rightarrow> equation_term * equation_term"
+definition CC_union :: "(equation \<Rightarrow> bool) \<Rightarrow> equation \<Rightarrow> equation \<Rightarrow> bool"
   where
-"equation_\<alpha> (a \<approx> b) = (Symb a, Symb b)"
-| "equation_\<alpha> (F a b \<approx> c) = (Apply (Symb a) (Symb b), Symb c)"
+"CC_union CC eq' = Congruence_Closure ({eq | eq. CC eq} \<union> {eq'})"
 
-fun CC_union :: "(equation \<Rightarrow> bool) \<Rightarrow> (equation_term * equation_term) \<Rightarrow> (equation_term * equation_term) \<Rightarrow> bool"
-  where
-"CC_union CC (a, b) (a', b') = Congruence_Closure ({equation_\<alpha> eq | eq. CC eq} \<union> {(a, b)}) (a', b')"
+lemma Congruence_Closure_union:
+"Congruence_Closure S eqt \<Longrightarrow> Congruence_Closure (S \<union> S') eqt"
+  apply(induction rule: Congruence_Closure.induct)
+  using base apply blast
+  using reflexive apply blast
+  using symmetric apply blast
+  using transitive apply blast
+  using monotonic apply blast
+  done
+
+lemma CC_union_correct: 
+"CC_union (Congruence_Closure S) eq' eq = Congruence_Closure (S \<union> {eq'}) eq"
+proof
+  show "CC_union (Congruence_Closure S) eq' eq \<Longrightarrow> Congruence_Closure (S \<union> {eq'}) eq"
+    unfolding CC_union_def
+    apply(induction "{eqa |eqa. Congruence_Closure S eqa} \<union> {eq'}" eq rule: Congruence_Closure.induct)
+    using base Congruence_Closure_union apply blast
+    using reflexive apply blast
+    using symmetric apply blast
+    using transitive apply blast
+    using monotonic apply blast
+    done
+next
+  show "Congruence_Closure (S \<union> {eq'}) eq \<Longrightarrow> CC_union (Congruence_Closure S) eq' eq"
+    apply(induction "S \<union> {eq'}" eq rule: Congruence_Closure.induct)
+    unfolding CC_union_def 
+    using base apply auto[1]
+    using reflexive apply auto[1]
+    using symmetric apply auto[1]
+    using transitive apply blast
+    using monotonic apply blast
+    done
+qed
+
 
 fun valid_vars :: "equation \<Rightarrow> nat \<Rightarrow> bool"
   where
@@ -42,10 +72,60 @@ definition cc_\<alpha> :: "congruence_closure \<Rightarrow> equation \<Rightarro
   where
 "cc_\<alpha> cc x \<equiv> valid_vars x (nr_vars cc) \<and> are_congruent cc x"
 
-text \<open>TODO\<close>
+
+subsection \<open>Invariants\<close>
+text \<open>As described in the paper\<close>
+
+text \<open>For cc_list_invar we use ufa_invar\<close>
+
+text \<open>for each representative i, UseList (i) is a list of input equations \<open>f(b\<^sub>1, b\<^sub>2)=b\<close>
+such that i is the representative of \<open>b\<^sub>1\<close> or of \<open>b\<^sub>2\<close> (or of both).\<close>
+definition use_list_invar :: "congruence_closure \<Rightarrow> bool"
+  where
+"use_list_invar cc = (\<forall> i < nr_vars cc . (\<forall> j < length ((use_list cc) ! i) . 
+(cc_list cc) ! i = i \<longrightarrow> (\<exists> b\<^sub>1 b\<^sub>2 b .
+use_list cc ! i ! j = (F b\<^sub>1 b\<^sub>2 \<approx> b) \<and> 
+(i = rep_of (cc_list cc) b\<^sub>1) \<or> i = rep_of (cc_list cc) b\<^sub>2)))"
+
+text \<open>for all pairs of representatives (i, j), Lookup(i, j) is some input equation
+\<open>f(a\<^sub>1, a\<^sub>2)=a\<close> such that i and j are the current respective representatives of \<open>a\<^sub>1\<close> and \<open>a\<^sub>2\<close> whenever
+such an equation exists. Otherwise, Lookup(i, j) is \<bottom>\<close>
+definition lookup_invar :: "congruence_closure \<Rightarrow> bool"
+  where
+"lookup_invar cc = (\<forall> i < nr_vars cc . (\<forall> j < nr_vars cc . 
+(cc_list cc) ! i = i \<and> (cc_list cc) ! j = j \<longrightarrow>
+lookup cc ! i ! j = None \<or> (\<exists> a\<^sub>1 a\<^sub>2 a . lookup cc ! i ! j = Some (F a\<^sub>1 a\<^sub>2 \<approx> a) \<and> 
+rep_of (cc_list cc) a\<^sub>1 = i \<and> rep_of (cc_list cc) a\<^sub>2 = j)))"
+
+definition representativeE :: "congruence_closure \<Rightarrow> equation set"
+  where
+"representativeE cc = {a \<approx> rep_of (cc_list cc) a |a.  a < nr_vars cc \<and> cc_list cc ! a \<noteq> a}
+\<union> {F a' b' \<approx> rep_of (cc_list cc) c | a' b' c c\<^sub>1 c\<^sub>2 . a' < nr_vars cc \<and> b' < nr_vars cc \<and> c < nr_vars cc \<and>
+                      cc_list cc ! a' = a' \<and> cc_list cc ! b' = b' \<and> lookup cc ! a' ! b' = Some (F c\<^sub>1 c\<^sub>2 \<approx> c)}"
+
+text \<open>TODO: 
+Inv1: RepresentativeE is in standard form;
+A set of equations E is in standard form if its equations are of the form a = b or
+of the form f(a, b) = c whose (respective) left hand side terms a and f(a, b) only occur once
+in E.\<close>
+definition inv1 :: "congruence_closure \<Rightarrow> bool"
+  where
+"inv1 cc = True"
+
+definition inv2 :: "congruence_closure \<Rightarrow> bool"
+  where
+"inv2 cc \<equiv> 
+Congruence_Closure (representativeE cc) = Congruence_Closure (set (input cc))"
+
+lemma cc_\<alpha>_eq_CC_representativeE: "cc_\<alpha> cc (s \<approx> t) = Congruence_Closure (representativeE cc) (s \<approx> t)"
+  sorry
+
 abbreviation cc_invar :: "congruence_closure \<Rightarrow> bool"
   where
-"cc_invar cc \<equiv> True"
+"cc_invar cc \<equiv> use_list_invar cc \<and> lookup_invar cc \<and> inv1 cc \<and> inv2 cc"
+
+lemma cc_invar_initial_cc: "cc_invar (initial_cc n)"
+  sorry
 
 text \<open>The length of all arrays of congruence_closure is always nr_vars cc\<close>
 lemma length_initial_cc:
@@ -87,27 +167,86 @@ lemma propagate_preserves_length_use_list:
 
 lemma propagate_preserves_length_lookup:
   assumes "propagate_dom (a, cc)" "length (lookup cc) = n" 
-(*"add_edge_dom(proof_forest cc, a, b)"*)
   shows "length (lookup (propagate a cc)) = n"
   using assms apply(induction rule: propagate.pinduct)
   unfolding propagate.psimps Let_def
-  sorry
+  using set_lookup_preserves_length
+  by auto
 
 lemma propagate_preserves_length_proof_forest:
   assumes "propagate_dom (a, cc)" "length (proof_forest cc) = n "
   shows "length (proof_forest (propagate a cc)) = n"
-  using assms apply(induction rule: propagate.pinduct)
-  unfolding propagate.psimps Let_def
-  sorry
+  using assms proof(induction rule: propagate.pinduct)
+  case (1 cc)
+  then show ?case 
+    by (simp add: propagate.psimps(1))
+next
+  case (2 pe xs l u t pf pfl ip)
+  define a where "a = left pe"
+  define b where "b = right pe"
+  have "add_edge_dom (pf, a, b)"
+    sorry
+  with 2 add_edge_preserves_length a_def b_def show ?case 
+    by (smt (verit) congruence_closure.select_convs(4) propagate.psimps(2))
+qed
 
 lemma propagate_preserves_length_pf_labels:
-  assumes "propagate_dom (a, cc)" "length (pf_labels cc) = n "
+  assumes "propagate_dom (a, cc)" "length (pf_labels cc) = n"
   shows "length (pf_labels (propagate a cc)) = n"
-  using assms apply(induction rule: propagate.pinduct)
-  unfolding propagate.psimps Let_def
-  sorry
+  using assms proof(induction rule: propagate.pinduct)
+  case (1 cc)
+  then show ?case 
+    by (simp add: propagate.psimps(1))
+next
+  case (2 pe xs l u t pf pfl ip)
+  define a where "a = left pe"
+  have "add_label_dom (pfl, pf, a, pe)"
+    sorry
+  with 2 add_label_preserves_length a_def propagate.psimps(2) show ?case 
+    by (smt (verit) congruence_closure.select_convs(5) )
+qed
+thm "add_edge_rel.intros"
+thm "rep_of_rel.intros"
+lemma add_edge_rel: "rep_of_rel (l, x) (l, y) \<longleftrightarrow> add_edge_rel (l[y := y'], x, y) (l, y, y')" 
+proof
+  show "rep_of_rel (l, x) (l, y) \<Longrightarrow> add_edge_rel (l[y := y'], x, y) (l, y, y')"
+    by (induction "(l, x)" "(l, y)" rule: rep_of_rel.induct)(auto simp add: add_edge_rel.intros)
+next
+  show "add_edge_rel (l[y := y'], x, y) (l, y, y') \<Longrightarrow> rep_of_rel (l, x) (l, y)"
+    by (induction "(l[y := y'], x, y)" "(l, y, y')" rule: add_edge_rel.induct) (auto simp add: rep_of_rel.intros)
+qed
+thm add_edge.domintros
 
-
+lemma "add_edge_dom (l, l ! i, x) \<Longrightarrow> add_edge_dom (l[i := y'], l ! i, x)"
+proof(induction l "l!i" x arbitrary: x rule: add_edge.pinduct)
+  case (1 pf e e')
+  have "pf[i := y'] ! e = e \<Longrightarrow> add_edge_dom (pf[i := y'], e, x)" using add_edge.domintros by blast
+  from 1 have *: "add_edge_dom (pf[pf ! i := e, i := y'], pf[pf ! i := e] ! i, e')" sorry
+  have "pf[pf ! i := e] ! i = pf ! i" "pf[pf ! i := e, i := y'] = pf[i := y']" sorry
+  with * show ?case 
+    by argo
+qed
+lemma add_edge_dom: "ufa_invar l \<Longrightarrow> y < length l \<Longrightarrow> add_edge_dom (l, y, y')"
+proof(induction arbitrary: y' rule: rep_of_induct)
+  case (base i)
+  then show ?case 
+    using add_edge.domintros by blast
+next
+  case (step i)
+  have "add_edge_dom (l[i := y'], l ! i, i)"
+    sorry
+  then show ?case 
+    using add_edge.domintros by blast
+qed
+proof
+lemma "ufa_invar pf \<Longrightarrow> a < length pf \<Longrightarrow> add_edge_dom (pf, a, b)"
+proof(induction rule: rep_of_induct)
+  case (base i)
+  then show ?case using add_edge.psimps sorry
+next
+  case (step i)
+  then show ?case sorry
+qed
 
 
 
