Congruence_Closure_Explain/Congruence_Closure_Proofs.thy
@@ -14,15 +14,32 @@ lemma "CC_union (cc_\<alpha> cc) (equation_\<alpha> eq) (equation_\<alpha> eq') 
   sorry
 
 lemma 
-"valid_vars eq n \<Longrightarrow>
+"valid_vars eq n \<Longrightarrow> 
 cc_\<alpha> (apply_merges (initial_cc n) xs) eq = Congruence_Closure (equation_\<alpha> ` set xs) (equation_\<alpha> eq)"
   sorry
 
+subsection \<open>Correctness of merge v2\<close>
+
+lemma 
+"valid_vars eq n \<Longrightarrow> cc_invar cc \<Longrightarrow> 
+cc_\<alpha> (apply_merges (initial_cc n) xs) eq = Congruence_Closure_v2 (set xs) eq"
+  sorry
+lemma 
+"valid_vars eq n \<Longrightarrow> cc_invar cc \<Longrightarrow> 
+cc_\<alpha> cc eq = Congruence_Closure_v2 (set (input cc)) eq"
+  sorry
+
 subsection \<open>Correctness of are_congruent\<close>
-
-
+lemma "valid_vars eq (nr_vars cc) \<Longrightarrow> are_congruent cc eq = cc_\<alpha> cc eq"
+  unfolding cc_\<alpha>_def by simp
 
 subsection \<open>Correctness of explain\<close>
+lemma "are_congruent cc (a \<approx> b) \<Longrightarrow> cc_invar cc \<Longrightarrow>
+  Congruence_Closure (equation_\<alpha> ` (cc_explain cc ([0..<nr_vars cc]) [(a,b)])) (Symb a, Symb b)"
+  sorry
 
+lemma "are_congruent cc (a \<approx> b) \<Longrightarrow> cc_invar cc \<Longrightarrow>
+  Congruence_Closure_v2 (cc_explain cc ([0..<nr_vars cc]) [(a, b)]) (a \<approx> b)"
+  sorry
 
 end 
